lean4/BEDC.lean
@@ -35,3 +35,5 @@ import BEDC.Derived.BoolUp
 import BEDC.Derived.OptionUp
 import BEDC.Derived.ProdUp
 import BEDC.Derived.ListUp
+import BEDC.Derived.SumUp
+import BEDC.Derived.MonoidUp
